implement simple quantifier heuristics
The quantifier heuristics library is powerful, but often slow. The
unwind conversions are fast, but have serious restrictions. This commits
adds simple quantifier heuristics. They are based on the techniques
developed for quantifier heuristics library, but only search gap guesses
that don't contain free variables. Some very limited experiments suggest
that it is similarly fast as unwind. It can handle all the cases unwind
can handle. However, it supports also a much richer syntax. Moreover, it
can instantiate in addition to universal and existential quantifiers
also unique existential quantifiers, eliminate select and some.
Moreover, it knows about pairs and lists.

src/quantHeuristics/quantHeuristicsScript.sml
@@ -734,6 +734,152 @@ val IMP_NEG_CONTRA = store_thm("IMP_NEG_CONTRA",
 val DISJ_IMP_INTRO  = store_thm ("DISJ_IMP_INTRO",
   ``(!x. P x \/ Q x) ==> ((~(P y) ==> Q y) /\ (~(Q y) ==> P y))``, PROVE_TAC[])
 
+
+(******************************************************************************)
+(* Simple GUESSES                                                             *)
+(******************************************************************************)
+
+val SIMPLE_GUESS_EXISTS_def = Define `
+    SIMPLE_GUESS_EXISTS (v : 'a) (i : 'a) (P : bool) =
+      (P ==> (v = i))`
+
+val SIMPLE_GUESS_EXISTS_ALT_DEF = store_thm ("SIMPLE_GUESS_EXISTS_ALT_DEF",
+  ``(!v. SIMPLE_GUESS_EXISTS (v:'a) i (P v)) <=> (
+    GUESS_EXISTS_GAP ((K i):(unit -> 'a)) (\v. P v))``,
+SIMP_TAC std_ss [SIMPLE_GUESS_EXISTS_def, GUESS_EXISTS_GAP_def]);
+
+
+val SIMPLE_GUESS_FORALL_def = Define `
+    SIMPLE_GUESS_FORALL (v : 'a) (i : 'a) (P : bool) =
+      (~P ==> (v = i))`
+
+val SIMPLE_GUESS_FORALL_ALT_DEF = store_thm ("SIMPLE_GUESS_FORALL_ALT_DEF",
+  ``(!v. SIMPLE_GUESS_FORALL (v:'a) i (P v)) <=> (
+    GUESS_FORALL_GAP ((K i):(unit -> 'a)) (\v. P v))``,
+SIMP_TAC std_ss [SIMPLE_GUESS_FORALL_def, GUESS_FORALL_GAP_def]);
+
+val SIMPLE_GUESS_FORALL_THM = store_thm ("SIMPLE_GUESS_FORALL_THM",
+  ``!i P. (!v. SIMPLE_GUESS_FORALL v i (P v)) ==>
+    ((!v. P v) <=> (P i))``,
+REWRITE_TAC [SIMPLE_GUESS_FORALL_def] THEN
+METIS_TAC[])
+
+val SIMPLE_GUESS_EXISTS_THM = store_thm ("SIMPLE_GUESS_EXISTS_THM",
+  ``!i P. (!v. SIMPLE_GUESS_EXISTS v i (P v)) ==>
+    ((?v. P v) <=> (P i))``,
+REWRITE_TAC [SIMPLE_GUESS_EXISTS_def] THEN
+METIS_TAC[])
+
+val SIMPLE_GUESS_UEXISTS_THM = store_thm ("SIMPLE_GUESS_UEXISTS_THM",
+  ``!i P.
+    (!v. SIMPLE_GUESS_EXISTS v i (P v)) ==>
+    ((?!v. P v) <=> (P i))``,
+SIMP_TAC std_ss [SIMPLE_GUESS_EXISTS_def, EXISTS_UNIQUE_THM] THEN
+METIS_TAC[])
+
+val SIMPLE_GUESS_SELECT_THM = store_thm ("SIMPLE_GUESS_SELECT_THM",
+  ``!i P.
+    (!v. SIMPLE_GUESS_EXISTS v i (P v)) ==>
+    ((@v. P v) = if P i then i else (@v. F))``,
+SIMP_TAC std_ss [SIMPLE_GUESS_EXISTS_def] THEN
+REPEAT STRIP_TAC THEN
+Cases_on `P i` THEN ASM_REWRITE_TAC [] THENL [
+  SELECT_ELIM_TAC THEN
+  METIS_TAC[],
+
+  `!v. P v = F` by METIS_TAC[] THEN
+  ASM_REWRITE_TAC[]
+])
+
+
+val SIMPLE_GUESS_SOME_THM = store_thm ("SIMPLE_GUESS_SOME_THM",
+  ``!i P.
+    (!v. SIMPLE_GUESS_EXISTS v i (P v)) ==>
+    ((some v. P v) = (if P i then SOME i else NONE))``,
+
+SIMP_TAC std_ss [SIMPLE_GUESS_EXISTS_def, some_def] THEN
+REPEAT STRIP_TAC THEN
+Cases_on `?v. P v` THEN (
+  ASM_REWRITE_TAC [] THEN
+  METIS_TAC[]
+))
+
+val SIMPLE_GUESS_TAC =
+  SIMP_TAC std_ss [SIMPLE_GUESS_FORALL_def, SIMPLE_GUESS_EXISTS_def] THEN METIS_TAC[];
+
+val SIMPLE_GUESS_EXISTS_EQ_1 = store_thm ("SIMPLE_GUESS_EXISTS_EQ_1",
+  ``!v:'a i. SIMPLE_GUESS_EXISTS v i (v = i)``,
+  SIMPLE_GUESS_TAC)
+
+val SIMPLE_GUESS_EXISTS_EQ_2 = store_thm ("SIMPLE_GUESS_EXISTS_EQ_2",
+  ``!v:'a i. SIMPLE_GUESS_EXISTS v i (i = v)``,
+  SIMPLE_GUESS_TAC)
+
+val SIMPLE_GUESS_EXISTS_EQ_T = store_thm ("SIMPLE_GUESS_EXISTS_EQ_T",
+  ``!v. SIMPLE_GUESS_EXISTS v T v``,
+  SIMPLE_GUESS_TAC)
+
+val SIMPLE_GUESS_FORALL_NEG = store_thm ("SIMPLE_GUESS_FORALL_NEG",
+  ``!v:'a i P. SIMPLE_GUESS_EXISTS v i P ==> SIMPLE_GUESS_FORALL v i (~P)``,
+  SIMPLE_GUESS_TAC
+)
+
+val SIMPLE_GUESS_EXISTS_NEG = store_thm ("SIMPLE_GUESS_EXISTS_NEG",
+  ``!v:'a i P. SIMPLE_GUESS_FORALL v i P ==> SIMPLE_GUESS_EXISTS v i (~P)``,
+  SIMPLE_GUESS_TAC
+)
+
+val SIMPLE_GUESS_FORALL_OR_1 = store_thm ("SIMPLE_GUESS_FORALL_OR_1",
+  ``!v:'a i P1 P2. SIMPLE_GUESS_FORALL v i P1 ==> SIMPLE_GUESS_FORALL v i (P1 \/ P2)``,
+  SIMPLE_GUESS_TAC);
+
+val SIMPLE_GUESS_FORALL_OR_2 = store_thm ("SIMPLE_GUESS_FORALL_OR_2",
+  ``!v:'a i P1 P2. SIMPLE_GUESS_FORALL v i P2 ==> SIMPLE_GUESS_FORALL v i (P1 \/ P2)``,
+  SIMPLE_GUESS_TAC);
+
+val SIMPLE_GUESS_EXISTS_AND_1 = store_thm ("SIMPLE_GUESS_EXISTS_AND_1",
+  ``!v:'a i P1 P2. SIMPLE_GUESS_EXISTS v i P1 ==> SIMPLE_GUESS_EXISTS v i (P1 /\ P2)``,
+  SIMPLE_GUESS_TAC);
+
+val SIMPLE_GUESS_EXISTS_AND_2 = store_thm ("SIMPLE_GUESS_EXISTS_AND_2",
+  ``!v:'a i P1 P2. SIMPLE_GUESS_EXISTS v i P2 ==> SIMPLE_GUESS_EXISTS v i (P1 /\ P2)``,
+  SIMPLE_GUESS_TAC);
+
+val SIMPLE_GUESS_EXISTS_EXISTS = store_thm ("SIMPLE_GUESS_EXISTS_EXISTS",
+  ``!v:'a i P. (!v2. SIMPLE_GUESS_EXISTS v i (P v2)) ==>
+               SIMPLE_GUESS_EXISTS v i (?v2. P v2)``,
+  SIMPLE_GUESS_TAC)
+
+val SIMPLE_GUESS_EXISTS_FORALL = store_thm ("SIMPLE_GUESS_EXISTS_FORALL",
+  ``!v:'a i P. (!v2. SIMPLE_GUESS_EXISTS v i (P v2)) ==>
+               SIMPLE_GUESS_EXISTS v i (!v2. P v2)``,
+  SIMPLE_GUESS_TAC)
+
+val SIMPLE_GUESS_FORALL_EXISTS = store_thm ("SIMPLE_GUESS_FORALL_EXISTS",
+  ``!v:'a i P. (!v2. SIMPLE_GUESS_FORALL v i (P v2)) ==>
+               SIMPLE_GUESS_FORALL v i (?v2. P v2)``,
+  SIMPLE_GUESS_TAC)
+
+val SIMPLE_GUESS_FORALL_FORALL = store_thm ("SIMPLE_GUESS_FORALL_FORALL",
+  ``!v i P. (!v2. SIMPLE_GUESS_FORALL v i (P v2)) ==>
+            SIMPLE_GUESS_FORALL v i (!v2. P v2)``,
+  SIMPLE_GUESS_TAC)
+
+val SIMPLE_GUESS_FORALL_IMP_1 = store_thm ("SIMPLE_GUESS_FORALL_IMP_1",
+  ``!v:'a i P1 P2. SIMPLE_GUESS_EXISTS v i P1 ==> SIMPLE_GUESS_FORALL v i (P1 ==> P2)``,
+  SIMPLE_GUESS_TAC);
+
+val SIMPLE_GUESS_FORALL_IMP_2 = store_thm ("SIMPLE_GUESS_FORALL_IMP_2",
+  ``!v:'a i P1 P2. SIMPLE_GUESS_FORALL v i P2 ==> SIMPLE_GUESS_FORALL v i (P1 ==> P2)``,
+  SIMPLE_GUESS_TAC);
+
+val SIMPLE_GUESS_EXISTS_EQ_FUN = store_thm ("SIMPLE_GUESS_EXISTS_EQ_FUN",
+  ``!v:'a i t1 t2 f.
+      SIMPLE_GUESS_EXISTS v i (f t1 = f t2) ==>
+      SIMPLE_GUESS_EXISTS v i (t1 = t2)``,
+  SIMPLE_GUESS_TAC)
+
+
 (******************************************************************************)
 (* Removing functions under quantifiers                                       *)
 (******************************************************************************)
